automation fixes

stdlib/rr_internal/theories/shims.v
@@ -188,7 +188,14 @@ Next Obligation. solve_fn_vars_nodup. Qed.
 Definition size_of_array_in_bytes `{!LayoutAlg} (st : syn_type) (len : nat) : nat :=
   let ly := use_layout_alg' st in
   ly.(ly_size) * len.
-Global Hint Unfold size_of_array_in_bytes : solve_goal_unfold.
+Local Hint Unfold size_of_array_in_bytes : solve_goal_unfold.
+
+Lemma size_of_array_in_bytes_mono `{!LayoutAlg} st (len1 len2 : nat) :
+  len1 ≤ len2 →
+  size_of_array_in_bytes st len1 ≤ size_of_array_in_bytes st len2.
+Proof.
+  unfold size_of_array_in_bytes. nia.
+Qed.
 
 (** alloc_array *)
 Program Definition alloc_array `{!LayoutAlg} (T_st : syn_type) (mem_align_log_of_T_loc : loc) (mem_size_of_T_loc : loc) (alloc_alloc_loc : loc) : function := {|
